chore: move to new frontend

src/Init/WF.lean
@@ -1,3 +1,4 @@
+#lang lean4
 /-
 Copyright (c) 2014 Microsoft Corporation. All rights reserved.
 Released under Apache 2.0 license as described in the file LICENSE.
@@ -11,144 +12,175 @@ universes u v
 set_option codegen false
 
 inductive Acc {α : Sort u} (r : α → α → Prop) : α → Prop
-| intro (x : α) (h : ∀ y, r y x → Acc y) : Acc x
+| intro (x : α) (h : (y : α) → r y x → Acc r y) : Acc r x
 
 @[elabAsEliminator, inline, reducible]
 def Acc.ndrec.{u1, u2} {α : Sort u2} {r : α → α → Prop} {C : α → Sort u1}
-    (m : ∀ (x : α) (h : ∀ (y : α), r y x → Acc r y), (∀ (y : α) (a : r y x), C y) → C x)
+    (m : (x : α) → ((y : α) → r y x → Acc r y) → ((y : α) → (a : r y x) → C y) → C x)
     {a : α} (n : Acc r a) : C a :=
-@Acc.rec α r (fun α _ => C α) m a n
+Acc.rec (motive := fun α _ => C α) m n
 
 @[elabAsEliminator, inline, reducible]
 def Acc.ndrecOn.{u1, u2} {α : Sort u2} {r : α → α → Prop} {C : α → Sort u1}
     {a : α} (n : Acc r a)
-    (m : ∀ (x : α) (h : ∀ (y : α), r y x → Acc r y), (∀ (y : α) (a : r y x), C y) → C x)
+    (m : (x : α) → ((y : α) → r y x → Acc r y) → ((y : α) → (a : r y x) → C y) → C x)
     : C a :=
-@Acc.rec α r (fun α _ => C α) m a n
+Acc.rec (motive := fun α _ => C α) m n
 
 namespace Acc
 variables {α : Sort u} {r : α → α → Prop}
 
 def inv {x y : α} (h₁ : Acc r x) (h₂ : r y x) : Acc r y :=
-Acc.recOn h₁ (fun x₁ ac₁ ih h₂ => ac₁ y h₂) h₂
+Acc.recOn (motive := fun (x : α) _ => r y x → Acc r y)
+  h₁ (fun x₁ ac₁ ih h₂ => ac₁ y h₂) h₂
 
 end Acc
 
 inductive WellFounded {α : Sort u} (r : α → α → Prop) : Prop
-| intro (h : ∀ a, Acc r a) : WellFounded
+  | intro (h : ∀ a, Acc r a) : WellFounded r
 
 class HasWellFounded (α : Sort u) : Type u :=
-(r : α → α → Prop) (wf : WellFounded r)
+  (r : α → α → Prop)
+  (wf : WellFounded r)
 
 namespace WellFounded
-def apply {α : Sort u} {r : α → α → Prop} (wf : WellFounded r) : ∀ a, Acc r a :=
-fun a => WellFounded.recOn wf (fun p => p) a
+def apply {α : Sort u} {r : α → α → Prop} (wf : WellFounded r) (a : α) : Acc r a :=
+  WellFounded.recOn (motive := fun x => (y : α) → Acc r y)
+    wf (fun p => p) a
 
 section
 variables {α : Sort u} {r : α → α → Prop} (hwf : WellFounded r)
 
-theorem recursion {C : α → Sort v} (a : α) (h : ∀ x, (∀ y, r y x → C y) → C x) : C a :=
-Acc.recOn (apply hwf a) (fun x₁ ac₁ ih => h x₁ ih)
+theorem recursion {C : α → Sort v} (a : α) (h : ∀ x, (∀ y, r y x → C y) → C x) : C a := by
+  induction (apply hwf a) with
+  | intro x₁ ac₁ ih => exact h x₁ ih
 
 theorem induction {C : α → Prop} (a : α) (h : ∀ x, (∀ y, r y x → C y) → C x) : C a :=
-recursion hwf a h
+  recursion hwf a h
 
 variable {C : α → Sort v}
 variable (F : ∀ x, (∀ y, r y x → C y) → C x)
 
-def fixF (x : α) (a : Acc r x) : C x :=
-Acc.recOn a (fun x₁ ac₁ ih => F x₁ ih)
+def fixF (x : α) (a : Acc r x) : C x := by
+  induction a with
+  | intro x₁ ac₁ ih => exact F x₁ ih
 
-theorem fixFEq (x : α) (acx : Acc r x) :
-  fixF F x acx = F x (fun (y : α) (p : r y x) => fixF F y (Acc.inv acx p)) :=
-Acc.rec (fun x r ih => rfl) acx
+def fixFEq (x : α) (acx : Acc r x) : fixF F x acx = F x (fun (y : α) (p : r y x) => fixF F y (Acc.inv acx p)) := by
+  induction acx with
+  | intro x r ih => exact rfl
+
 end
 
 variables {α : Sort u} {C : α → Sort v} {r : α → α → Prop}
 
 -- Well-founded fixpoint
 def fix (hwf : WellFounded r) (F : ∀ x, (∀ y, r y x → C y) → C x) (x : α) : C x :=
-fixF F x (apply hwf x)
+  fixF F x (apply hwf x)
 
 -- Well-founded fixpoint satisfies fixpoint equation
 theorem fixEq (hwf : WellFounded r) (F : ∀ x, (∀ y, r y x → C y) → C x) (x : α) :
-  fix hwf F x = F x (fun y h => fix hwf F y) :=
-fixFEq F x (apply hwf x)
+    fix hwf F x = F x (fun y h => fix hwf F y) :=
+  fixFEq F x (apply hwf x)
 end WellFounded
 
 open WellFounded
 
 -- Empty relation is well-founded
-def emptyWf {α : Sort u} : WellFounded (@emptyRelation α) :=
-WellFounded.intro (fun (a : α) =>
-  Acc.intro a (fun (b : α) (lt : False) => False.rec _ lt))
+def emptyWf {α : Sort u} : WellFounded (@emptyRelation α) := by
+  apply WellFounded.intro
+  intro a
+  apply Acc.intro a
+  intro b h
+  cases h
 
 -- Subrelation of a well-founded relation is well-founded
 namespace Subrelation
 variables {α : Sort u} {r q : α → α → Prop}
 
-def accessible {a : α} (h₁ : Subrelation q r) (ac : Acc r a) : Acc q a :=
-Acc.recOn ac $ fun x ax ih =>
-  Acc.intro x $ fun (y : α) (lt : q y x) => ih y (h₁ lt)
+def accessible {a : α} (h₁ : Subrelation q r) (ac : Acc r a) : Acc q a := by
+  induction ac with
+  | intro x ax ih =>
+    apply Acc.intro
+    intro y h
+    exact ih y (h₁ h)
 
 def wf (h₁ : Subrelation q r) (h₂ : WellFounded r) : WellFounded q :=
-⟨fun a => accessible @h₁ (apply h₂ a)⟩
+  ⟨fun a => accessible @h₁ (apply h₂ a)⟩
 end Subrelation
 
 -- The inverse image of a well-founded relation is well-founded
 namespace InvImage
 variables {α : Sort u} {β : Sort v} {r : β → β → Prop}
 
-private def accAux (f : α → β) {b : β} (ac : Acc r b) : ∀ (x : α), f x = b → Acc (InvImage r f) x :=
-Acc.ndrecOn ac $ fun x acx ih z e =>
-  Acc.intro z  $ fun y lt =>
-    Eq.ndrecOn e (fun acx ih => ih (f y) lt y rfl) acx ih
+private def accAux (f : α → β) {b : β} (ac : Acc r b) : (x : α) → f x = b → Acc (InvImage r f) x := by
+  induction ac with
+  | intro x acx ih =>
+    intro z e
+    apply Acc.intro
+    intro y lt
+    subst x
+    apply ih (f y) lt y rfl
 
 def accessible {a : α} (f : α → β) (ac : Acc r (f a)) : Acc (InvImage r f) a :=
-accAux f ac a rfl
+  accAux f ac a rfl
 
 def wf (f : α → β) (h : WellFounded r) : WellFounded (InvImage r f) :=
-⟨fun a => accessible f (apply h (f a))⟩
+  ⟨fun a => accessible f (apply h (f a))⟩
 end InvImage
 
 -- The transitive closure of a well-founded relation is well-founded
 namespace TC
 variables {α : Sort u} {r : α → α → Prop}
 
-def accessible {z : α} (ac : Acc r z) : Acc (TC r) z :=
-Acc.ndrecOn ac $ fun x acx ih =>
-  Acc.intro x $ fun y rel =>
-    TC.ndrecOn rel
-      (fun a b rab acx ih => ih a rab)
-      (fun a b c rab rbc ih₁ ih₂ acx ih => Acc.inv (ih₂ acx ih) rab)
-      acx ih
+def accessible {z : α} (ac : Acc r z) : Acc (TC r) z := by
+  induction ac with
+  | intro x acx ih =>
+    apply Acc.intro x
+    intro y rel
+    revert acx ih
+    induction rel with
+    | base a b rab => intro acx ih; exact ih a rab
+    | trans a b c rab rbc ih₁ ih₂ =>
+      intro acx ih
+      apply Acc.inv (ih₂ acx ih) rab
 
 def wf (h : WellFounded r) : WellFounded (TC r) :=
-⟨fun a => accessible (apply h a)⟩
+  ⟨fun a => accessible (apply h a)⟩
 end TC
 
 -- less-than is well-founded
-def Nat.ltWf : WellFounded Nat.lt :=
-⟨Nat.rec
-  (Acc.intro 0 (fun n h => absurd h (Nat.notLtZero n)))
-  (fun n ih => Acc.intro (Nat.succ n) $ fun m h =>
-     Or.elim (Nat.eqOrLtOfLe (Nat.leOfSuccLeSucc h))
-        (fun e => Eq.substr e ih) (Acc.inv ih))⟩
+def Nat.ltWf : WellFounded Nat.lt := by
+  apply WellFounded.intro
+  intro n
+  induction n with
+  | zero      =>
+    apply Acc.intro 0
+    intro _ h
+    apply absurd h (Nat.notLtZero _)
+  | succ n ih =>
+    apply Acc.intro (Nat.succ n)
+    intro m h
+    have m = n ∨ m < n from Nat.eqOrLtOfLe (Nat.leOfSuccLeSucc h)
+    match this with
+    | Or.inl e => subst e; assumption
+    | Or.inr e => exact Acc.inv ih e
 
 def measure {α : Sort u} : (α → Nat) → α → α → Prop :=
-InvImage (fun a b => a < b)
+  InvImage (fun a b => a < b)
 
 def measureWf {α : Sort u} (f : α → Nat) : WellFounded (measure f) :=
-InvImage.wf f Nat.ltWf
+  InvImage.wf f Nat.ltWf
 
 def sizeofMeasure (α : Sort u) [HasSizeof α] : α → α → Prop :=
-measure sizeof
+  measure sizeof
 
 def sizeofMeasureWf (α : Sort u) [HasSizeof α] : WellFounded (sizeofMeasure α) :=
-measureWf sizeof
+  measureWf sizeof
 
-instance hasWellFoundedOfHasSizeof (α : Sort u) [HasSizeof α] : HasWellFounded α :=
-{r := sizeofMeasure α, wf := sizeofMeasureWf α}
+instance hasWellFoundedOfHasSizeof (α : Sort u) [HasSizeof α] : HasWellFounded α := {
+  r := sizeofMeasure α,
+  wf := sizeofMeasureWf α
+}
 
 namespace Prod
 open WellFounded
@@ -160,44 +192,52 @@ variable  (rb  : β → β → Prop)
 
 -- Lexicographical order based on ra and rb
 inductive Lex : α × β → α × β → Prop
-| left  {a₁} (b₁) {a₂} (b₂) (h : ra a₁ a₂) : Lex (a₁, b₁) (a₂, b₂)
-| right (a) {b₁ b₂} (h : rb b₁ b₂)         : Lex (a, b₁)  (a, b₂)
+  | left  {a₁} (b₁) {a₂} (b₂) (h : ra a₁ a₂) : Lex (a₁, b₁) (a₂, b₂)
+  | right (a) {b₁ b₂} (h : rb b₁ b₂)         : Lex (a, b₁)  (a, b₂)
 
 -- relational product based on ra and rb
 inductive Rprod : α × β → α × β → Prop
-| intro {a₁ b₁ a₂ b₂} (h₁ : ra a₁ a₂) (h₂ : rb b₁ b₂) : Rprod (a₁, b₁) (a₂, b₂)
+  | intro {a₁ b₁ a₂ b₂} (h₁ : ra a₁ a₂) (h₂ : rb b₁ b₂) : Rprod (a₁, b₁) (a₂, b₂)
 end
 
 section
 variables {α : Type u} {β : Type v}
 variables {ra  : α → α → Prop} {rb  : β → β → Prop}
 
-def lexAccessible {a} (aca : Acc ra a) (acb : ∀ b, Acc rb b): ∀ b, Acc (Lex ra rb) (a, b) :=
-Acc.ndrecOn aca $ fun xa aca iha b =>
-  Acc.ndrecOn (acb b) $ fun xb acb ihb =>
-    Acc.intro (xa, xb)  $ fun p lt =>
-      have aux : xa = xa → xb = xb → Acc (Lex ra rb) p from
-        @Prod.Lex.recOn α β ra rb (fun p₁ p₂ _ => fst p₂ = xa → snd p₂ = xb → Acc (Lex ra rb) p₁)
-                         p (xa, xb) lt
-          (fun (a₁ b₁ a₂ b₂ h) (Eq₂ : a₂ = xa) (Eq₃ : b₂ = xb) => iha a₁ (Eq.recOn Eq₂ h) b₁)
-          (fun (a b₁ b₂ h) (Eq₂ : a = xa) (Eq₃ : b₂ = xb) => Eq.recOn Eq₂.symm (ihb b₁ (Eq.recOn Eq₃ h)));
-      aux rfl rfl
+def lexAccessible {a} (aca : Acc ra a) (acb : ∀ b, Acc rb b) (b : β) : Acc (Lex ra rb) (a, b) := by
+  revert b
+  induction aca with
+  | intro xa aca iha =>
+    intro b
+    induction (acb b) with
+    | intro xb acb ihb =>
+      apply Acc.intro (xa, xb)
+      intro p lt
+      cases lt with
+      | left  a₁ b₁ a₂ b₂ h => apply iha a₁ h
+      | right a b₁ b₂ h     => apply ihb b₁ h
 
 -- The lexicographical order of well founded relations is well-founded
 def lexWf (ha : WellFounded ra) (hb : WellFounded rb) : WellFounded (Lex ra rb) :=
-⟨fun p => casesOn p $ fun a b => lexAccessible (apply ha a) (WellFounded.apply hb) b⟩
+  ⟨fun (a, b) => lexAccessible (apply ha a) (WellFounded.apply hb) b⟩
 
 -- relational product is a Subrelation of the Lex
-def rprodSubLex : ∀ a b, Rprod ra rb a b → Lex ra rb a b :=
-@Prod.Rprod.rec _ _ ra rb (fun a b _ => Lex ra rb a b) (fun a₁ b₁ a₂ b₂ h₁ h₂ => Lex.left b₁ b₂ h₁)
+def rprodSubLex (a : α × β) (b : α × β) (h : Rprod ra rb a b) : Lex ra rb a b := by
+  cases h with
+  | intro a₁ b₁ a₂ b₂ h₁ h₂ => exact Lex.left b₁ b₂ h₁
 
 -- The relational product of well founded relations is well-founded
-def rprodWf (ha : WellFounded ra) (hb : WellFounded rb) : WellFounded (Rprod ra rb) :=
-Subrelation.wf (rprodSubLex) (lexWf ha hb)
+def rprodWf (ha : WellFounded ra) (hb : WellFounded rb) : WellFounded (Rprod ra rb) := by
+  apply Subrelation.wf (r := Lex ra rb) (h₂ := lexWf ha hb)
+  intro a b h
+  exact rprodSubLex a b h
+
 end
 
-instance HasWellFounded {α : Type u} {β : Type v} [s₁ : HasWellFounded α] [s₂ : HasWellFounded β] : HasWellFounded (α × β) :=
-{r := Lex s₁.r s₂.r, wf := lexWf s₁.wf s₂.wf}
+instance {α : Type u} {β : Type v} [s₁ : HasWellFounded α] [s₂ : HasWellFounded β] : HasWellFounded (α × β) := {
+  r  := Lex s₁.r s₂.r,
+  wf := lexWf s₁.wf s₂.wf
+}
 
 end Prod
 
@@ -209,52 +249,40 @@ variable  (s  : ∀ a, β a → β a → Prop)
 
 -- Lexicographical order based on r and s
 inductive Lex : PSigma β → PSigma β → Prop
-| left  : ∀ {a₁ : α} (b₁ : β a₁) {a₂ : α} (b₂ : β a₂), r a₁ a₂ → Lex ⟨a₁, b₁⟩ ⟨a₂, b₂⟩
-| right : ∀ (a : α)  {b₁ b₂ : β a}, s a b₁ b₂ → Lex ⟨a, b₁⟩ ⟨a, b₂⟩
+  | left  : ∀ {a₁ : α} (b₁ : β a₁) {a₂ : α} (b₂ : β a₂), r a₁ a₂ → Lex ⟨a₁, b₁⟩ ⟨a₂, b₂⟩
+  | right : ∀ (a : α)  {b₁ b₂ : β a}, s a b₁ b₂ → Lex ⟨a, b₁⟩ ⟨a, b₂⟩
 end
 
 section
 variables {α : Sort u} {β : α → Sort v}
 variables {r  : α → α → Prop} {s : ∀ (a : α), β a → β a → Prop}
 
-def lexAccessible {a} (aca : Acc r a) (acb : ∀ a, WellFounded (s a)) : ∀ (b : β a), Acc (Lex r s) ⟨a, b⟩ :=
-Acc.ndrecOn aca $ fun (xa aca) (iha : ∀ y, r y xa → ∀ (b : β y), Acc (Lex r s) ⟨y, b⟩) (b : β xa) =>
-  Acc.ndrecOn (WellFounded.apply (acb xa) b) $ fun xb acb (ihb : ∀ (y : β xa), s xa y xb → Acc (Lex r s) ⟨xa, y⟩) =>
-     Acc.intro ⟨xa, xb⟩ $ fun (p) (lt : Lex r s p ⟨xa, xb⟩) =>
-        have aux : xa = xa → xb ≅ xb → Acc (Lex r s) p from
-          @PSigma.Lex.recOn α β r s (fun p₁ p₂ _ => p₂.1 = xa → p₂.2 ≅ xb → Acc (Lex r s) p₁)
-                            p ⟨xa, xb⟩ lt
-            (fun (a₁ : α) (b₁ : β a₁) (a₂ : α) (b₂ : β a₂) (h : r a₁ a₂) (Eq₂ : a₂ = xa) (Eq₃ : b₂ ≅ xb) =>
-              have aux : (∀ (y : α), r y xa → ∀ (b : β y), Acc (Lex r s) ⟨y, b⟩) →
-                         r a₁ a₂ → ∀ (b₁ : β a₁), Acc (Lex r s) ⟨a₁, b₁⟩ from Eq.subst Eq₂ (fun iha h b₁ => iha a₁ h b₁);
-              aux iha h b₁)
-            (fun (a : α) (b₁ b₂ : β a) (h : s a b₁ b₂) (Eq₂ : a = xa) (Eq₃ : b₂ ≅ xb) =>
-              have aux : ∀ (xb : β xa), (∀ (y : β xa), s xa y xb → Acc (s xa) y) →
-                           (∀ (y : β xa), s xa y xb → Acc (Lex r s) ⟨xa, y⟩) →
-                           Lex r s p ⟨xa, xb⟩ → ∀ (b₁ : β a), s a b₁ b₂ → b₂ ≅ xb → Acc (Lex r s) ⟨a, b₁⟩
-              from Eq.subst Eq₂ $ fun xb acb ihb lt b₁ h Eq₃ =>
-                have newEq₃ : b₂ = xb from eqOfHEq Eq₃;
-                have aux : (∀ (y : β a), s a y xb → Acc (Lex r s) ⟨a, y⟩) →
-                           ∀ (b₁ : β a), s a b₁ b₂ → Acc (Lex r s) ⟨a, b₁⟩
-                from Eq.subst newEq₃ (fun ihb b₁ h => ihb b₁ h);
-                aux ihb b₁ h;
-              aux xb acb ihb lt b₁ h Eq₃);
-        aux rfl (HEq.refl xb)
+def lexAccessible {a} (aca : Acc r a) (acb : (a : α) → WellFounded (s a)) (b : β a) : Acc (Lex r s) ⟨a, b⟩ := by
+  revert b
+  induction aca with
+  | intro xa aca iha =>
+    intro b
+    induction (WellFounded.apply (acb xa) b) with
+    | intro xb acb ihb =>
+      apply Acc.intro
+      intro p lt
+      cases lt with
+      | left  => apply iha; assumption
+      | right => apply ihb; assumption
 
 -- The lexicographical order of well founded relations is well-founded
-def lexWf (ha : WellFounded r) (hb : ∀ x, WellFounded (s x)) : WellFounded (Lex r s) :=
-WellFounded.intro $ fun ⟨a, b⟩ => lexAccessible (WellFounded.apply ha a) hb b
+def lexWf (ha : WellFounded r) (hb : (x : α) → WellFounded (s x)) : WellFounded (Lex r s) :=
+  WellFounded.intro fun ⟨a, b⟩ => lexAccessible (WellFounded.apply ha a) hb b
 end
 
 section
 variables {α : Sort u} {β : Sort v}
 
 def lexNdep (r : α → α → Prop) (s : β → β → Prop) :=
-Lex r (fun a => s)
+  Lex r (fun a => s)
 
-def lexNdepWf {r  : α → α → Prop} {s : β → β → Prop} (ha : WellFounded r) (hb : WellFounded s)
-                : WellFounded (lexNdep r s) :=
-WellFounded.intro $ fun ⟨a, b⟩ => lexAccessible (WellFounded.apply ha a) (fun x => hb) b
+def lexNdepWf {r  : α → α → Prop} {s : β → β → Prop} (ha : WellFounded r) (hb : WellFounded s) : WellFounded (lexNdep r s) :=
+    WellFounded.intro $ fun ⟨a, b⟩ => lexAccessible (WellFounded.apply ha a) (fun x => hb) b
 end
 
 section
@@ -262,8 +290,8 @@ variables {α : Sort u} {β : Sort v}
 
 -- Reverse lexicographical order based on r and s
 inductive RevLex (r  : α → α → Prop) (s  : β → β → Prop) : @PSigma α (fun a => β) → @PSigma α (fun a => β) → Prop
-| left  : ∀ {a₁ a₂ : α} (b : β), r a₁ a₂ → RevLex ⟨a₁, b⟩ ⟨a₂, b⟩
-| right : ∀ (a₁ : α) {b₁ : β} (a₂ : α) {b₂ : β}, s b₁ b₂ → RevLex ⟨a₁, b₁⟩ ⟨a₂, b₂⟩
+| left  : {a₁ a₂ : α} → (b : β) → r a₁ a₂ → RevLex r s ⟨a₁, b⟩ ⟨a₂, b⟩
+| right : (a₁ : α) → {b₁ : β} → (a₂ : α) → {b₂ : β} → s b₁ b₂ → RevLex r s ⟨a₁, b₁⟩ ⟨a₂, b₂⟩
 end
 
 section
@@ -271,40 +299,36 @@ open WellFounded
 variables {α : Sort u} {β : Sort v}
 variables {r  : α → α → Prop} {s : β → β → Prop}
 
-def revLexAccessible {b} (acb : Acc s b) (aca : ∀ a, Acc r a): ∀ a, Acc (RevLex r s) ⟨a, b⟩ :=
-Acc.recOn acb $ fun (xb acb) (ihb : ∀ y, s y xb → ∀ a, Acc (RevLex r s) ⟨a, y⟩) (a) =>
-  Acc.recOn (aca a) $ fun (xa aca) (iha : ∀ y, r y xa → Acc (RevLex r s) (mk y xb)) =>
-    Acc.intro ⟨xa, xb⟩ $ fun (p) (lt : RevLex r s p ⟨xa, xb⟩) =>
-      have aux : xa = xa → xb = xb → Acc (RevLex r s) p from
-        @RevLex.recOn α β r s (fun p₁ p₂ _ => fst p₂ = xa → snd p₂ = xb → Acc (RevLex r s) p₁)
-                            p ⟨xa, xb⟩ lt
-          (fun (a₁ a₂ b) (h : r a₁ a₂) (Eq₂ : a₂ = xa) (Eq₃ : b = xb) =>
-             show Acc (RevLex r s) ⟨a₁, b⟩ from
-             have r₁ : r a₁ xa from Eq.recOn Eq₂ h;
-             have aux : Acc (RevLex r s) ⟨a₁, xb⟩ from iha a₁ r₁;
-             Eq.recOn (Eq.symm Eq₃) aux)
-          (fun (a₁ b₁ a₂ b₂) (h : s b₁ b₂) (Eq₂ : a₂ = xa) (Eq₃ : b₂ = xb) =>
-            show Acc (RevLex r s) (mk a₁ b₁) from
-            have s₁ : s b₁ xb from Eq.recOn Eq₃ h;
-            ihb b₁ s₁ a₁);
-      aux rfl rfl
+def revLexAccessible {b} (acb : Acc s b) (aca : (a : α) → Acc r a): (a : α) → Acc (RevLex r s) ⟨a, b⟩ := by
+  induction acb with
+  | intro xb acb ihb =>
+    intro a
+    induction (aca a) with
+    | intro xa aca iha =>
+      apply Acc.intro
+      intro p lt
+      cases lt with
+      | left  => apply iha; assumption
+      | right => apply ihb; assumption
 
 def revLexWf (ha : WellFounded r) (hb : WellFounded s) : WellFounded (RevLex r s) :=
-WellFounded.intro $ fun ⟨a, b⟩ => revLexAccessible (apply hb b) (WellFounded.apply ha) a
+  WellFounded.intro $ fun ⟨a, b⟩ => revLexAccessible (apply hb b) (WellFounded.apply ha) a
 end
 
 section
 def skipLeft (α : Type u) {β : Type v} (s : β → β → Prop) : @PSigma α (fun a => β) → @PSigma α (fun a => β) → Prop :=
-RevLex emptyRelation s
+  RevLex emptyRelation s
 
 def skipLeftWf (α : Type u) {β : Type v} {s : β → β → Prop} (hb : WellFounded s) : WellFounded (skipLeft α s) :=
-revLexWf emptyWf hb
+  revLexWf emptyWf hb
 
 def mkSkipLeft {α : Type u} {β : Type v} {b₁ b₂ : β} {s : β → β → Prop} (a₁ a₂ : α) (h : s b₁ b₂) : skipLeft α s ⟨a₁, b₁⟩ ⟨a₂, b₂⟩ :=
-RevLex.right _ _ h
+  RevLex.right _ _ h
 end
 
-instance HasWellFounded {α : Type u} {β : α → Type v} [s₁ : HasWellFounded α] [s₂ : ∀ a, HasWellFounded (β a)] : HasWellFounded (PSigma β) :=
-{r := Lex s₁.r (fun a => (s₂ a).r), wf := lexWf s₁.wf (fun a => (s₂ a).wf)}
+instance HasWellFounded {α : Type u} {β : α → Type v} [s₁ : HasWellFounded α] [s₂ : ∀ a, HasWellFounded (β a)] : HasWellFounded (PSigma β) := {
+  r  := Lex s₁.r (fun a => (s₂ a).r),
+  wf := lexWf s₁.wf (fun a => (s₂ a).wf)
+}
 
 end PSigma
